A very first version of the MOSI protocol

src/Ex/Mosi/Mosi.v
@@ -11,6 +11,678 @@ Local Open Scope list.
 Local Open Scope hvec.
 Local Open Scope fmap.
 
+(** Design choices:
+ * - Multi-level (for arbitrary tree structure)
+ * - MOSI
+ * - Directory (not snooping)
+ * - Invalidate (not update)
+ * - Write-back (not write-through)
+ * - NINE (non-inclusive non-exclusive)
+ *)
+
 Section System.
+  Variable (tr: tree).
+
+  Definition topo := fst (tree2Topo tr 0).
+  Definition cifc := snd (tree2Topo tr 0).
+  Opaque topo cifc.
+  
+  Definition implValueIdx: Fin.t 3 := F1.
+  Definition implStatusIdx: Fin.t 3 := F2.
+  Definition implDirIdx: Fin.t 3 := F3.
+
+  Section Directory.
+    
+    Record DirT: Set :=
+      { dir_st: MOSI; (* the summary status for children *)
+        dir_owner: IdxT; (* the owner has a status either M or O *)
+        dir_sharers: list IdxT
+      }.
+
+    Definition dirInit: DirT :=
+      {| dir_st := mosiS;
+         dir_owner := ii;
+         dir_sharers := nil (** FIXME: should be children indices. *) |}.
+
+    Import CaseNotations.
+    Definition getDir (oidx: IdxT) (dir: DirT): MOSI :=
+      match case dir.(dir_st) on eq_nat_dec default mosiI with
+      | mosiM: if idx_dec oidx dir.(dir_owner) then mosiM else mosiI
+      | mosiO: if idx_dec oidx dir.(dir_owner) then mosiO else mosiI
+      | mosiS: if in_dec idx_dec oidx dir.(dir_sharers)
+               then mosiS else mosiI
+      | mosiI: mosiI
+      end.
+
+    Definition setDirM (oidx: IdxT) :=
+      {| dir_st := mosiM;
+         dir_owner := oidx;
+         dir_sharers := nil |}.
+
+    Definition setDirO (oidx: IdxT) :=
+      {| dir_st := mosiO;
+         dir_owner := oidx;
+         dir_sharers := [oidx] |}.
+
+    Definition setDirS (oinds: list IdxT) :=
+      {| dir_st := mosiS;
+         dir_owner := ii;
+         dir_sharers := oinds |}.
+    
+    Definition setDirI :=
+      {| dir_st := mosiI;
+         dir_owner := ii;
+         dir_sharers := nil |}.
+
+    Definition addSharer (oidx: IdxT) (dir: DirT): DirT :=
+      {| dir_st := dir.(dir_st);
+         dir_owner := dir.(dir_owner);
+         dir_sharers := oidx :: dir.(dir_sharers) |}.
+    
+    Definition removeSharer (oidx: IdxT) (dir: DirT): DirT :=
+      {| dir_st := dir.(dir_st);
+         dir_owner := dir.(dir_owner);
+         dir_sharers := removeOnce idx_dec oidx dir.(dir_sharers) |}.
+
+    Definition removeOwner (oidx: IdxT) (dir: DirT): DirT :=
+      {| dir_st := mosiS;
+         dir_owner := ii;
+         dir_sharers := removeOnce idx_dec oidx dir.(dir_sharers) |}.
+    
+  End Directory.
+
+  Instance ImplOStateIfc: OStateIfc :=
+    {| ost_ty := [nat:Type; MOSI:Type; DirT:Type]%vector |}.
+
+  Definition implOStateInit: OState :=
+    (0, (mosiS, (dirInit, tt))).
+  
+  Definition implOStatesInit: OStates :=
+    fold_left (fun m i => m +[i <- implOStateInit])
+              (cifc.(c_l1_indices) ++ cifc.(c_li_indices)) [].
+
+  Definition implORqsInit: ORqs Msg :=
+    initORqs (cifc.(c_l1_indices) ++ cifc.(c_li_indices)).
+
+  (** A core idea: a "summary" status in each object *)
+
+  Definition summaryOf (ost: OState): MOSI :=
+    if Compare_dec.le_gt_dec mosiS ost#[implStatusIdx]
+    then ost#[implStatusIdx]
+    else ost#[implDirIdx].(dir_st).
+
+  Section Rules.
+    Variables (oidx cidx: IdxT).
+
+    Section GetTrs.
+
+      Definition l1GetSImm: Rule :=
+        rule.immd[cidx~>0~>0]
+        :accepts mosiRqS
+        :from cidx
+        :requires (fun ost orq mins => mosiS <= ost#[implStatusIdx])
+        :transition
+           (!|ost, _| --> (ost, {| miv_id := mosiRsS;
+                                   miv_value := ost#[implValueIdx]
+                                |})).
+
+      Definition liGetSImmOS: Rule :=
+        rule.immd[cidx~>0~>0~>0]
+        :accepts mosiRqS
+        :from cidx
+        :requires
+           (fun ost orq mins =>
+              ost#[implStatusIdx] = mosiS \/ ost#[implStatusIdx] = mosiO)
+        :transition
+           (!|ost, _| --> (ost, {| miv_id := mosiRsS;
+                                   miv_value := ost#[implValueIdx]
+                                |})).
+
+      Definition liGetSImmM: Rule :=
+        rule.immd[cidx~>0~>0~>1]
+        :accepts mosiRqS
+        :from cidx
+        :requires (fun ost orq mins => ost#[implStatusIdx] = mosiM)
+        :transition
+           (!|ost, _| --> (ost +#[implStatusIdx <- mosiO]
+                               +#[implDirIdx <- setDirS [cidx]],
+                           {| miv_id := mosiRsS;
+                              miv_value := ost#[implValueIdx]
+                           |})).
+
+      (** NOTE (common rules): some rules do not require distinguishing L1 and Li 
+       * caches. In correctness proof we may have to prove invariants, e.g., the
+       * directory status of L1 is always [mosiI] since it does not have children.
+       *)
+
+      (* commonly used *)
+      Definition getSRqUpUp: Rule :=
+        rule.rquu[cidx~>0~>1]
+        :accepts mosiRqS
+        :from cidx
+        :me oidx
+        :requires (fun ost mins => summaryOf ost = mosiI)
+        :transition (!|ost, msg| --> {| miv_id := mosiRqS; miv_value := O |}).
+
+      Definition l1GetSRsDownDownS: Rule :=
+        rule.rsdd[0~>2]
+        :accepts mosiRsS
+        :holding mosiRqS
+        :requires ⊤
+        :transition
+           (!|ost, min, rq, rsbTo|
+            --> (ost +#[implValueIdx <- msg_value min]
+                     +#[implStatusIdx <- mosiS],
+                 {| miv_id := mosiRsS;
+                    miv_value := msg_value min |})).
+
+      Definition liGetSRsDownDownS: Rule :=
+        rule.rsdd[0~>2]
+        :accepts mosiRsS
+        :holding mosiRqS
+        :requires ⊤
+        :transition
+           (!|ost, min, rq, rsbTo|
+            --> (ost +#[implDirIdx <- setDirS [objIdxOf rsbTo]],
+                 {| miv_id := mosiRsS;
+                    miv_value := msg_value min |})).
+
+      Definition liGetSRqUpDownS: Rule :=
+        rule.rqud[cidx~>0~>3~>0]
+        :accepts mosiRqS
+        :from cidx
+        :me oidx
+        :requires
+           (fun ost mins =>
+              and (ost#[implStatusIdx] = mosiI)
+                  (ost#[implDirIdx].(dir_st) = mosiS))
+        :transition
+           (!|ost, msg| --> ([hd ii (ost#[implDirIdx].(dir_sharers))],
+                             {| miv_id := mosiDownRqS;
+                                miv_value := O |})).
+
+      Definition liGetSRqUpDownMO: Rule :=
+        rule.rqud[cidx~>0~>3]
+        :accepts mosiRqS
+        :from cidx
+        :me oidx
+        :requires
+           (fun ost mins =>
+              and (ost#[implStatusIdx] = mosiI)
+                  (mosiS <= ost#[implDirIdx].(dir_st)))
+        :transition
+           (!|ost, msg| --> ([ost#[implDirIdx].(dir_owner)],
+                             {| miv_id := mosiDownRqS;
+                                miv_value := O |})).
+
+      (* commonly used *)
+      Definition downSImmS: Rule :=
+        rule.immu[0~>4~>0]
+        :accepts mosiDownRqS
+        :me oidx
+        :requires (fun ost orq mins => ost#[implStatusIdx] = mosiS)
+        :transition
+           (!|ost, min| --> (ost, {| miv_id := mosiDownRsS;
+                                     miv_value := ost#[implValueIdx] |})).
+
+      (* commonly used *)
+      Definition downSImmMO: Rule :=
+        rule.immu[0~>4~>1]
+        :accepts mosiDownRqS
+        :me oidx
+        :requires (fun ost orq mins => mosiO <= ost#[implStatusIdx])
+        :transition
+           (!|ost, min| --> (ost +#[implStatusIdx <- mosiO],
+                             {| miv_id := mosiDownRsS;
+                                miv_value := ost#[implValueIdx] |})).
+
+      Definition liDownSRsUpDownS: Rule :=
+        rule.rsud[0~>5~>0]
+        :accepts mosiDownRsS
+        :holding mosiRqS
+        :requires
+           (FirstMsg /\ (fun ost orq mins => ost#[implDirIdx].(dir_st) = mosiS))
+        :transition
+           (!|ost, mins, rq, rssFrom, rsbTo|
+            --> (msg ::= getFirstMsgI mins;
+                 rsFrom ::= getFirstIdxFromI rssFrom;
+                 (ost, {| miv_id := mosiRsS;
+                          miv_value := msg_value msg |}))).
+
+      Definition liDownSRsUpDownMO: Rule :=
+        rule.rsud[0~>5~>1]
+        :accepts mosiDownRsS
+        :holding mosiRqS
+        :requires
+           (FirstMsg /\ (fun ost orq mins => mosiO <= ost#[implDirIdx].(dir_st)))
+        :transition
+           (!|ost, mins, rq, rssFrom, rsbTo|
+            --> (msg ::= getFirstMsgI mins;
+                 rsFrom ::= getFirstIdxFromI rssFrom;
+                 (ost +#[implDirIdx
+                           <- addSharer (objIdxOf rsbTo) (setDirO (objIdxOf rsFrom))],
+                  {| miv_id := mosiRsS;
+                     miv_value := msg_value msg |}))).
+
+      Definition liDownSRqDownDownS: Rule :=
+        rule.rqdd[0~>6~>0]
+        :accepts mosiDownRqS
+        :me oidx
+        :requires
+           (fun ost mins =>
+              and (ost#[implStatusIdx] = mosiI)
+                  (ost#[implDirIdx].(dir_st) = mosiS))
+        :transition
+           (!|ost, msg| --> ([hd ii (ost#[implDirIdx].(dir_sharers))],
+                             {| miv_id := mosiDownRqS;
+                                miv_value := O |})).
+
+      Definition liDownSRqDownDownMO: Rule :=
+        rule.rqdd[0~>6~>1]
+        :accepts mosiDownRqS
+        :me oidx
+        :requires
+           (fun ost mins =>
+              and (ost#[implStatusIdx] = mosiI)
+                  (mosiO <= ost#[implDirIdx].(dir_st)))
+        :transition
+           (!|ost, msg| --> ([ost#[implDirIdx].(dir_owner)],
+                             {| miv_id := mosiDownRqS;
+                                miv_value := O |})).
+
+      Definition liDownSRsUpUpS: Rule :=
+        rule.rsuu[0~>7~>0]
+        :accepts mosiDownRsS
+        :holding mosiDownRqS
+        :requires
+           (FirstMsg /\ (fun ost orq mins => ost#[implDirIdx].(dir_st) = mosiS))
+        :transition
+           (!|ost, mins, rq, rssFrom, rsbTo|
+            --> (msg ::= getFirstMsgI mins;
+                 rsFrom ::= getFirstIdxFromI rssFrom;
+                 (ost, {| miv_id := mosiDownRsS;
+                          miv_value := msg_value msg |}))).
+
+      Definition liDownSRsUpUpMO: Rule :=
+        rule.rsuu[0~>7~>1]
+        :accepts mosiDownRsS
+        :holding mosiDownRqS
+        :requires
+           (FirstMsg /\ (fun ost orq mins => mosiO <= ost#[implDirIdx].(dir_st)))
+        :transition
+           (!|ost, mins, rq, rssFrom, rsbTo|
+            --> (msg ::= getFirstMsgI mins;
+                 rsFrom ::= getFirstIdxFromI rssFrom;
+                 (ost +#[implDirIdx <- setDirO (objIdxOf rsFrom)],
+                  {| miv_id := mosiRsS;
+                     miv_value := msg_value msg |}))).
+
+    End GetTrs.
+
+    Section SetTrs.
+
+      Definition l1GetMImm: Rule :=
+        rule.immd[cidx~>1~>0]
+        :accepts mosiRqM
+        :from cidx
+        :requires (fun ost orq mins => ost#[implStatusIdx] = mosiM)
+        :transition
+           (!|ost, msg|
+            --> (ost +#[implValueIdx <- msg_value msg],
+                 {| miv_id := mosiRsM;
+                    miv_value := O |})).
+
+      Definition liGetMImm: Rule :=
+        rule.immd[cidx~>1~>0]
+        :accepts mosiRqM
+        :from cidx
+        :requires (fun ost orq mins => ost#[implStatusIdx] = mosiM)
+        :transition
+           (!|ost, msg| --> (ost +#[implStatusIdx <- mosiI]
+                                 +#[implDirIdx <- setDirM cidx],
+                             {| miv_id := mosiRsM;
+                                miv_value := O |})).
+
+      (* commonly used *)
+      Definition getMRqUpUp: Rule :=
+        rule.rquu[cidx~>1~>1]
+        :accepts mosiRqM
+        :from cidx
+        :me oidx
+        :requires (fun ost mins => summaryOf ost < mosiM)
+        :transition (!|ost, msg| --> {| miv_id := mosiRqM; miv_value := O |}).
+
+      Definition l1GetMRsDownDown: Rule :=
+        rule.rsdd[1~>2]
+        :accepts mosiRsM
+        :holding mosiRqM
+        :requires ⊤
+        :transition
+           (!|ost, min, rq, rsbTo|
+            --> (ost +#[implStatusIdx <- mosiM]
+                     +#[implValueIdx <- msg_value rq],
+                 {| miv_id := mosiRsM;
+                    miv_value := O |})).
+
+      (* This is the case where it's possible to directly respond a [mosiRsM]
+       * message back since there are no internal sharers to invalidate.
+       *)
+      Definition liGetMRsDownDownDirI: Rule :=
+        rule.rsdd[1~>3]
+        :accepts mosiRsM
+        :holding mosiRqM
+        :requires (fun ost orq mins => ost#[implDirIdx].(dir_st) = mosiI)
+        :transition
+           (!|ost, min, rq, rsbTo|
+            --> (ost +#[implStatusIdx <- mosiI]
+                     +#[implDirIdx <- setDirM (objIdxOf rsbTo)],
+                 {| miv_id := mosiRsM;
+                    miv_value := O |})).
+
+      (* This is the case where internal invalidation is required due to
+       * sharers. 
+       *)
+      Definition liGetMRsDownRqDownDirOS: Rule :=
+        rule.rsrq[1~>4]
+        :accepts mosiRsM
+        :holding mosiRqM
+        :me oidx
+        :requires (fun ost orq mins =>
+                     ost#[implDirIdx].(dir_st) = mosiO \/
+                     ost#[implDirIdx].(dir_st) = mosiS)
+        :transition
+           (!|ost, rq| --> (ost#[implDirIdx].(dir_sharers),
+                            {| miv_id := mosiDownRqI;
+                               miv_value := O |})).
+
+      Definition liGetMRqUpDownM: Rule :=
+        rule.rqud[cidx~>1~>5]
+        :accepts mosiRqM
+        :from cidx
+        :me oidx
+        :requires
+           (fun ost mins =>
+              and (ost#[implStatusIdx] = mosiI)
+                  (ost#[implDirIdx].(dir_st) = mosiM))
+        :transition
+           (!|ost, msg| --> ([ost#[implDirIdx].(dir_owner)],
+                             {| miv_id := mosiDownRqI;
+                                miv_value := O |})).
+
+      Definition liDownIRsUpDown: Rule :=
+        rule.rsud[1~>6]
+        :accepts mosiDownRsI
+        :holding mosiRqM
+        :requires ⊤
+        :transition
+           (!|ost, mins, rq, rssFrom, rsbTo|
+              --> (ost +#[implStatusIdx <- mosiI]
+                       +#[implDirIdx <- setDirM (objIdxOf rsbTo)],
+                   {| miv_id := mosiRsM;
+                      miv_value := O |})).
+
+      Definition l1DownIImm: Rule :=
+        rule.immu[1~>7]
+        :accepts mosiDownRqI
+        :me oidx
+        :requires (fun ost orq mins => mosiS <= ost#[implStatusIdx])
+        :transition
+           (!|ost, min| --> (ost +#[implStatusIdx <- mosiI],
+                              {| miv_id := mosiDownRsI;
+                                 miv_value := O |})).
+
+      Definition liDownIImm: Rule :=
+        rule.immu[1~>8]
+        :accepts mosiDownRqI
+        :me oidx
+        :requires (fun ost orq mins => ost#[implDirIdx].(dir_st) = mosiI)
+        :transition
+           (!|ost, min| --> (ost +#[implStatusIdx <- mosiI],
+                             {| miv_id := mosiDownRsI;
+                                miv_value := O |})).
+
+      Definition liDownIRqDownDownDirOS: Rule :=
+        rule.rqdd[1~>9]
+        :accepts mosiDownRqI
+        :me oidx
+        :requires (fun ost mins =>
+                     ost#[implDirIdx].(dir_st) = mosiS \/
+                     ost#[implDirIdx].(dir_st) = mosiO)
+        :transition
+           (!|ost, msg| --> (ost#[implDirIdx].(dir_sharers),
+                             {| miv_id := mosiDownRqI;
+                                miv_value := O |})).
+
+      Definition liDownIRqDownDownDirM: Rule :=
+        rule.rqdd[1~>10]
+        :accepts mosiDownRqI
+        :me oidx
+        :requires
+           (fun ost mins =>
+              and (ost#[implStatusIdx] = mosiI)
+                  (ost#[implDirIdx].(dir_st) = mosiM))
+        :transition
+           (!|ost, msg| --> ([ost#[implDirIdx].(dir_owner)],
+                              {| miv_id := mosiDownRqI;
+                                 miv_value := O |})).
+
+      Definition liDownIRsUpUp: Rule :=
+        rule.rsuu[1~>11]
+        :accepts mosiDownRsI
+        :holding mosiDownRqI
+        :requires ⊤
+        :transition
+           (!|ost, mins, rq, rssFrom, rsbTo|
+            --> (ost +#[implStatusIdx <- mosiI]
+                     +#[implDirIdx <- setDirI],
+                   {| miv_id := mosiDownRsI;
+                      miv_value := O |})).
+
+      Definition memGetMRqUpDown: Rule :=
+        rule.rqud[cidx~>1~>12]
+        :accepts mosiRqM
+        :from cidx
+        :me oidx
+        :requires (fun ost mins => ost#[implStatusIdx] < mosiM)
+        :transition
+           (!|ost, msg| --> (ost#[implDirIdx].(dir_sharers),
+                             {| miv_id := mosiDownRqI;
+                                miv_value := O |})).
+
+    End SetTrs.
+
+    Section EvictTrs.
+
+      Definition putRqUpUp: Rule :=
+        rule.rqu[2~>0]
+        :me oidx
+        :requires (fun ost mins => ost#[implStatusIdx] < mosiO)
+        :transition
+           (ost --> {| miv_id := mosiRqI;
+                       miv_value := O |}).
+
+      Definition putRqUpUpMO: Rule :=
+        rule.rqu[2~>1]
+        :me oidx
+        :requires (fun ost mins => mosiO <= ost#[implStatusIdx])
+        :transition
+           (ost --> {| miv_id := mosiRqI;
+                       miv_value := ost#[implValueIdx] |}).
+
+      Definition putRsDownDown: Rule :=
+        rule.rsd[2~>2]
+        :accepts mosiRsI
+        :holding mosiRqI
+        :requires ⊤
+        :transition (!|ost, _, _| --> ost +#[implStatusIdx <- mosiI]).
+
+      Definition liPutImmI: Rule :=
+        rule.immd[cidx~>2~>3]
+        :accepts mosiRqI
+        :from cidx
+        :requires (fun ost orq mins => getDir cidx ost#[implDirIdx] = mosiI)
+        :transition
+           (!|ost, _| --> (ost, {| miv_id := mosiRsI;
+                                   miv_value := O
+                                |})).
+
+      Definition liPutImmS: Rule :=
+        rule.immd[cidx~>2~>4]
+        :accepts mosiRqI
+        :from cidx
+        :requires (fun ost orq mins => getDir cidx ost#[implDirIdx] = mosiS)
+        :transition
+           (!|ost, _|
+              --> (ost +#[implDirIdx <- removeSharer cidx ost#[implDirIdx]],
+                   {| miv_id := mosiRsI;
+                      miv_value := O
+                   |})).
+
+      Definition memPutImmSNotLast: Rule :=
+        rule.immd[cidx~>2~>4~>0]
+        :accepts mosiRqI
+        :from cidx
+        :requires
+           ((fun ost orq mins => getDir cidx ost#[implDirIdx] = mosiS) /\
+            (fun ost orq mins => List.length ost#[implDirIdx].(dir_sharers) >= 2))
+        :transition
+           (!|ost, msg|
+              --> (ost +#[implDirIdx <- removeSharer cidx ost#[implDirIdx]],
+                   {| miv_id := mosiRsI;
+                      miv_value := O
+                   |})).
+
+      Definition memPutImmSLast: Rule :=
+        rule.immd[cidx~>2~>4~>1]
+        :accepts mosiRqI
+        :from cidx
+        :requires
+           ((fun ost orq mins => getDir cidx ost#[implDirIdx] = mosiS) /\
+            (fun ost orq mins => List.length ost#[implDirIdx].(dir_sharers) = 1))
+        :transition
+           (!|ost, msg| --> (ost +#[implStatusIdx <- mosiM]
+                                 +#[implDirIdx <- setDirI],
+                             {| miv_id := mosiRsI;
+                                miv_value := O
+                             |})).
+
+      Definition liPutImmO: Rule :=
+        rule.immd[cidx~>2~>5]
+        :accepts mosiRqI
+        :from cidx
+        :requires (fun ost orq mins => getDir cidx ost#[implDirIdx] = mosiO)
+        :transition
+           (!|ost, msg| --> (ost +#[implStatusIdx <- mosiO]
+                                 +#[implValueIdx <- msg_value msg]
+                                 +#[implDirIdx <- removeOwner cidx ost#[implDirIdx]],
+                             {| miv_id := mosiRsI;
+                                miv_value := O
+                             |})).
+
+      Definition liPutImmM: Rule :=
+        rule.immd[cidx~>2~>6]
+        :accepts mosiRqI
+        :from cidx
+        :requires (fun ost orq mins => getDir cidx ost#[implDirIdx] = mosiM)
+        :transition
+           (!|ost, msg|
+              --> (ost +#[implStatusIdx <- mosiM]
+                       +#[implValueIdx <- msg_value msg]
+                       +#[implDirIdx <- setDirI],
+                   {| miv_id := mosiRsI;
+                      miv_value := O |})).
+
+    End EvictTrs.
+
+  End Rules.
+
+  Section Objects.
+    Variable (oidx: IdxT).
+
+    Section L1.
+
+      Local Notation eidx := (l1ExtOf oidx).
+
+      Definition l1: Object :=
+        {| obj_idx := oidx;
+           obj_rules :=
+             [(** rules involved with [GetS] *)
+               l1GetSImm eidx; getSRqUpUp oidx eidx;
+                 l1GetSRsDownDownS; downSImmS oidx; downSImmMO oidx;
+                   (** rules involved with [GetM] *)
+                   l1GetMImm eidx; getMRqUpUp oidx eidx;
+                     l1GetMRsDownDown; l1DownIImm oidx;
+                       (** rules involved with [Put] *)
+                       putRqUpUp oidx; putRqUpUpMO oidx; putRsDownDown];
+           obj_rules_valid := ltac:(inds_valid_tac) |}.
+
+    End L1.
+
+    Definition liRulesFromChild (cidx: IdxT): list Rule :=
+      [liGetSImmOS cidx; liGetSImmM cidx; getSRqUpUp oidx cidx;
+         liGetSRqUpDownS oidx cidx; liGetSRqUpDownMO oidx cidx;
+           liGetMImm cidx; getMRqUpUp oidx cidx; liGetMRqUpDownM oidx cidx;
+             liPutImmI cidx; liPutImmS cidx;
+               liPutImmO cidx; liPutImmM cidx].
+
+    Definition liRulesFromChildren (coinds: list IdxT): list Rule :=
+      List.concat (map liRulesFromChild coinds).
+
+    Program Definition li: Object :=
+      {| obj_idx := oidx;
+         obj_rules :=
+           (liRulesFromChildren (subtreeChildrenIndsOf topo oidx))
+             ++ [(** rules involved with [GetS] *)
+               liGetSRsDownDownS; downSImmS oidx; downSImmMO oidx;
+                 liDownSRsUpDownS; liDownSRsUpDownMO;
+                 liDownSRqDownDownS oidx; liDownSRqDownDownMO oidx;
+                   liDownSRsUpUpS; liDownSRsUpUpMO;
+                   (** rules involved with [GetM] *)
+                     liGetMRsDownDownDirI; liGetMRsDownRqDownDirOS oidx;
+                       liDownIRsUpDown; liDownIImm oidx;
+                       liDownIRqDownDownDirOS oidx; liDownIRqDownDownDirM oidx;
+                         liDownIRsUpUp;
+                         (** rules involved with [Put] *)
+                         putRqUpUp oidx; putRqUpUpMO oidx; putRsDownDown];
+         obj_rules_valid := _ |}.
+    Next Obligation.
+    Admitted.
+
+    Definition memRulesFromChild (cidx: IdxT): list Rule :=
+      [liGetSImmOS cidx; liGetSImmM cidx;
+         liGetSRqUpDownS oidx cidx; liGetSRqUpDownMO oidx cidx;
+           liGetMImm cidx; memGetMRqUpDown oidx cidx;
+             liPutImmI cidx; liPutImmS cidx;
+               liPutImmO cidx; liPutImmM cidx].
+
+    Definition memRulesFromChildren (coinds: list IdxT): list Rule :=
+      List.concat (map memRulesFromChild coinds).
+             
+    Program Definition mem: Object :=
+      {| obj_idx := oidx;
+         obj_rules :=
+           (memRulesFromChildren (subtreeChildrenIndsOf topo oidx))
+             ++ [liDownSRsUpDownS; liDownSRsUpDownMO; liDownIRsUpDown];
+         obj_rules_valid := _ |}.
+    Next Obligation.
+    Admitted.
+    
+  End Objects.
+
+  Program Definition impl: System :=
+    {| sys_objs :=
+         (map li cifc.(c_li_indices)) ++ (map l1 cifc.(c_l1_indices));
+       sys_oinds_valid := _;
+       sys_minds := cifc.(c_minds);
+       sys_merqs := cifc.(c_merqs);
+       sys_merss := cifc.(c_merss);
+       sys_msg_inds_valid := _;
+       sys_oss_inits := implOStatesInit;
+       sys_orqs_inits := implORqsInit |}.
+  Next Obligation.
+  Admitted.
+  Next Obligation.
+  Admitted.
   
 End System.
+
